experiment/Experiment.Steel.Repr.Test.Extract.fst
@@ -1,7 +1,18 @@
 module Experiment.Steel.Repr.Test.Extract
 
+module M    = Experiment.Steel.Repr.M
+module U32  = FStar.UInt32
 module Test = Experiment.Steel.Repr.Test
 
+open Steel.Effect
 open Steel.Reference
 
-let test3 (r0 r1 : ref nat) = Test.test3_steel r0 r1
+
+let test3 (r0 r1 : ref U32.t)
+  : Steel unit
+      (M.vprop_of_list (Test.test3_mem r0 r1)) (fun x -> M.vprop_of_list (Test.test3_mem r0 r1))
+      (requires fun h0      ->
+        U32.v (M.rmem_sels (Test.test3_mem r0 r1) h0 0) < 42)
+      (ensures  fun h0 () h1 ->
+        U32.v (M.rmem_sels (Test.test3_mem r0 r1) h1 1) == U32.v (M.rmem_sels (Test.test3_mem r0 r1) h0 0) + 1)
+  = Test.test3_steel r0 r1 ()
