pure/Learn.Util.fsti
@@ -27,7 +27,7 @@ let eq2_trans #t (x z : t) (y : t) (p0 : squash (x == y)) (p1 : squash (y == z))
   = ()
 
 
-unfold
+inline_for_extraction unfold
 let cast (#a b : Type) (x : a) : Pure b (requires a == b) (ensures fun y -> y == x)
   = x
 
